Synchronization on the master version

Executions.thy
@@ -1,5 +1,5 @@
 theory Executions
-imports IOA "~~/src/HOL/Library/Sublist"
+imports "IOA" "~~/src/HOL/Library/Sublist"
 begin
 
 (* Author: Giuliano Losa. This theory is an adaptation of the one by Olaf Mueller found in 
@@ -9,108 +9,9 @@ context IOA begin
 
 declare Let_def[simp]
 
-definition cons_exec where
-  "cons_exec p e \<equiv> (fst e, (snd e)#p)"
-
-definition append_exec where
-  "append_exec e e' \<equiv> (fst e, (snd e)@(snd e'))"
-
-fun last_state where
-  "last_state (s,[]) = s"
-| "last_state (s,ps#p) = snd p"
-
 definition proj_exec  ("_ \<downharpoonright> _ _") where
   "proj_exec e i sig \<equiv> 
     (fst e i, map (\<lambda> p . (fst p, snd p i)) (filter (\<lambda> p . fst p \<in> actions sig) (snd e)))"
-
-lemma last_state_reachable:
-  fixes A e
-  assumes "is_exec_of A e"
-  shows "reachable A (last_state e)" using assms
-proof -
-  have "is_exec_of A e \<Longrightarrow> reachable A (last_state e)"
-  proof (induction "snd e" arbitrary: e)
-    case Nil
-    from Nil.prems have 1:"fst e \<in> start A" by (simp add:is_exec_of_def)
-    from Nil.hyps have 2:"last_state e = fst e" by (metis last_state.simps(1) surjective_pairing)
-    from 1 and 2 and Nil.hyps show ?case by (metis reachable_0)
-  next
-    case (Cons p ps e)
-    let ?e' = "(fst e, ps)"
-    have ih:"reachable A (last_state ?e')"
-    proof -
-      from Cons.prems and Cons.hyps(2) have "is_exec_of A ?e'"
-        by (metis IOA.IOA.cons_exec_def IOA.exec_frag_prefix IOA.is_exec_of_def fst_conv prod.collapse swap_simp) 
-      with Cons.hyps(1) show ?thesis by auto
-    qed
-    from Cons.prems and Cons.hyps(2) have "(last_state ?e')\<midarrow>(fst p)\<midarrow>A\<longrightarrow>(snd p)"
-      apply(simp add:IOA.is_exec_of_def)
-        by (metis Executions.IOA.last_state.simps(1) Executions.IOA.last_state.simps(2) IOA.is_exec_frag_of.simps(1) IOA.is_exec_frag_of.simps(2) neq_Nil_conv prod.collapse)
-    with ih and Cons.hyps(2) show ?case
-      by (metis Executions.IOA.last_state.simps(2) IOA.reachable_n prod.collapse) 
-  qed
-  thus ?thesis using assms by fastforce
-qed 
-
-lemma trans_from_last_state:
-  assumes "is_exec_frag_of A e" and "(last_state e)\<midarrow>a\<midarrow>A\<longrightarrow>s'"
-  shows "is_exec_frag_of A (cons_exec (a,s') e)"
-    using assms
-      by (metis Executions.IOA.cons_exec_def Executions.IOA.last_state.elims IOA.IOA.cons_exec_def IOA.IOA.last_state.simps(1) IOA.IOA.last_state.simps(2) IOA.trans_from_last_state) 
-
-lemma exec_frag_prefix:
-  fixes A p ps
-  assumes "is_exec_frag_of A (cons_exec p e)"
-  shows "is_exec_frag_of A e"
-    using assms
-      by (simp add: Executions.IOA.cons_exec_def IOA.IOA.cons_exec_def IOA.exec_frag_prefix) 
-
-lemma trace_same_ext:
-  fixes A B e
-  assumes "ext A = ext B"
-  shows "trace (ioa.asig A) e = trace (ioa.asig B) e" 
-  using assms by (auto simp add:trace_def)
-
-lemma trace_append_is_append_trace:
-  fixes e e' sig
-  shows "trace sig (append_exec e' e) = trace sig e' @ trace sig e"
-  by (simp add:append_exec_def trace_def schedule_def filter_act_def)
-
-lemma append_exec_frags_is_exec_frag:
-  fixes e e' A as
-  assumes "is_exec_frag_of A e'" and "last_state e = fst e'" 
-  and "is_exec_frag_of A e"
-  shows "is_exec_frag_of A (append_exec e e')"
-proof -
-  from assms show ?thesis 
-  proof (induct e' rule:is_exec_frag_of.induct)
-    case (1 s)
-    from "1.hyps" "1.prems"(1,2,3)
-    show ?case
-      by (metis (no_types, hide_lams) Executions.IOA.append_exec_def IOA.is_exec_frag_of.simps(1) append_Cons fst_conv fst_swap swap_simp)  
-  next
-    case (2 A s p)
-    print_cases
-    have "last_state e \<midarrow>(fst p)\<midarrow>A\<longrightarrow> snd p" using "2.prems"(1,2)  fstI by auto
-    hence "is_exec_frag_of A (fst e, (snd e)#p)" using "2.prems"(1,3)
-      by (metis Executions.IOA.cons_exec_def Executions.IOA.trans_from_last_state assms(3) prod.collapse) 
-    moreover 
-    have "append_exec e (s, [p]) = (fst e, (snd e)#p)" using "2.prems"(1,2)
-      by (simp add: Executions.IOA.append_exec_def)
-    ultimately 
-      show ?case by auto
-  next
-    case (3 A s)
-      thus ?case
-        by (simp add: Executions.IOA.append_exec_def append_Nil prod.collapse snd_conv)
-  qed
-qed
-
-lemma last_state_of_append:
-  fixes e e'
-  assumes "fst e' = last_state e"
-  shows "last_state (append_exec e e') = last_state e'"
-  using assms by (cases e' rule:last_state.cases, auto simp add:append_exec_def)
 
 section {* Composition is monotonic with respect to the implementation relation *}
 
@@ -125,32 +26,32 @@ proof -
   proof (induction "snd e" arbitrary: e) 
     case Nil show ?case 
       by (simp add:proj_exec_def)
-      (metis Executions.IOA.last_state.simps(1) Nil.hyps filter.simps(1) list.simps(8) prod.collapse) 
+      (metis last_state.simps(1) Nil.hyps filter.simps(1) list.simps(8) prod.collapse) 
   next 
-    case (Cons p ps e)
+    case (Cons p ps e) print_cases
     from "Cons.prems" have 1:"is_exec_frag_of (par fam) (fst e, ps)"
-      by (metis Cons.hyps(2) Executions.IOA.cons_exec_def Executions.IOA.exec_frag_prefix prod.collapse snd_conv swap_simp)
+      by (metis Cons.hyps(2) is_exec_frag_of.simps(1) is_exec_frag_of.simps(3) list.exhaust surjective_pairing)
     from 1 and "Cons.hyps"
       have 2:"(last_state (fst e, ps)) i = last_state ((fst e, ps) \<downharpoonright> i (ioa.asig (memb fam i)))" 
         by simp
     show ?case
     proof (cases "fst p \<in> act (memb fam i)")
       case True
-      hence "last_state (fst e, ps#p) i = last_state ((fst e, ps#p) \<downharpoonright> i (ioa.asig (memb fam i)))"
+      hence "last_state (fst e, p#ps) i = last_state ((fst e, p#ps) \<downharpoonright> i (ioa.asig (memb fam i)))"
         by (simp add:proj_exec_def)
       with Cons.hyps(2) show ?thesis by simp
     next
       case False
-      from False have 3: "((fst e, ps#p) \<downharpoonright> i (ioa.asig (memb fam i))) 
+      from False have 3: "((fst e, p#ps) \<downharpoonright> i (ioa.asig (memb fam i))) 
                           = ((fst e, ps) \<downharpoonright> i (ioa.asig (memb fam i)))"
           by (simp add:proj_exec_def)
       from False and `i \<in> ids fam` and Cons.prems and Cons.hyps(2) 
-        have 4:"last_state (fst e, ps#p) i = last_state (fst e, ps) i" 
-          by (cases "(par fam, fst e, snd e)" rule:IOA.is_exec_frag_of.cases)
+        have 4:"last_state (fst e, p#ps) i = last_state (fst e, ps) i" 
+          by  (cases "(par fam, fst e, snd e)" rule:is_exec_frag_of.cases)
               (auto simp add:is_trans_def par_def)
       from 2 3 4 Cons.hyps(2) show ?thesis by simp
     qed
-  qed                                                     
+  qed
   with assms(2) show ?thesis by simp
 qed
 
@@ -169,15 +70,13 @@ proof -
     thus ?case by (simp add:proj_exec_def)
   next
     case (Cons p ps e)
-    let ?e = "(fst e, ps#p)"
+    let ?e = "(fst e, p#ps)"
     let ?e' = "(fst e, ps)"
     thm Cons.hyps
     from Cons.prems and Cons.hyps(2) have prems:"is_exec_frag_of (par fam) ?e" by simp
     from Cons.hyps have ih:"is_exec_frag_of (par fam) ?e' 
                           \<Longrightarrow> is_exec_frag_of A_i (?e' \<downharpoonright> i sig)" by simp
-    from prems have 0:"is_exec_frag_of (par fam) ?e'"
-      apply(simp add:par_def)
-      by (metis (lifting) IOA.IOA.cons_exec_def IOA.IOA.exec_frag_prefix fst_conv snd_conv)
+    from prems have 0:"is_exec_frag_of (par fam) ?e'" by (metis is_exec_frag_of.simps(1,3) list.exhaust)
     from 0 and ih have 1:"is_exec_frag_of A_i (?e' \<downharpoonright> i sig)" by auto
     have "is_exec_frag_of A_i (?e \<downharpoonright> i sig)"
     proof (cases "fst p \<in> act A_i")
@@ -188,9 +87,9 @@ proof -
       case True
       from True and prems and `i \<in> ids fam` 
         have 2:"(last_state ?e' i)\<midarrow>(fst p)\<midarrow>A_i\<longrightarrow>(snd p i)"
-          by (cases "(par fam, ?e')" rule:is_exec_frag_of.cases)
+          by  (cases "(par fam, ?e')" rule:is_exec_frag_of.cases)
               (auto simp add:A_i_def is_trans_def par_def split add:split_if_asm)
-      from True have 3:"(?e \<downharpoonright> i sig) = cons_exec (fst p, snd p i) (?e' \<downharpoonright> i sig)" 
+      from True have 3:"(?e \<downharpoonright> i sig) = cons_exec  (?e' \<downharpoonright> i sig) (fst p, snd p i)" 
         by (simp add:proj_exec_def A_i_def sig_def cons_exec_def)
       from `i \<in> ids fam` and last_state_proj and 0 
         have 4:"last_state ?e' i = last_state (?e' \<downharpoonright>i sig)" by (metis sig_def)
@@ -208,6 +107,6 @@ lemma paste_execs:
   assumes "\<forall> i \<in> ids fam . is_exec_of (memb fam i) (es i)"
     and "\<forall> i \<in> ids fam . let sig_i = ioa.asig (memb fam i) in (t \<bar> sig_i) = trace sig_i (es i)"
   obtains e where "is_exec_of (par fam) e" and "trace (ioa.asig (par fam)) e = t" 
-    and "\<forall> i \<in> ids fam . (e \<downharpoonright> i (ioa.asig (memb fam i))) = es i"
+    and "\<forall> i \<in> ids fam . (e \<downharpoonright> i (ioa.asig (memb fam i))) = es i" oops 
 
 end
